\documentclass[../../math.tex]{subfiles}
\externaldocument{../../math.tex}
\externaldocument{../basics/elementary_algebra}
\externaldocument{../basics/set}

\begin{document}

\setcounter{chapter}{7}

\chapter{The Rationals}

The rationals can be constructed from the integers by considering pairs of
integers $(a, b)$, thought of as the fraction $\frac{a}{b}$.  However, this
construction is more general than just for constructing the rationals from the
integers and applies to any integral domain.  Thus, in this chapter, most of the
construction will be using an arbitrary integral domain, and the rationals and
their unique properties won't be explored until the end.

\section{Basic Construction}

Let $\U$ be an integral domain, and let $\U^*$ be the type of all nonzero values
in $\U$.

\begin{definition}
    Define a relation $\sim$ on $\U \times \U^*$ where $(a_1, a_2) \sim (b_1,
    b_2)$ is defined to mean $a_1b_2 = b_1a_2$.
\end{definition}

\begin{lemma}
    The relation $\sim$ is an equivalence relation.
\end{lemma}
\begin{proof}
    \textit{Reflexivitity.}  We must check $a_1a_2 = a_1a_2$, which is a
    reflexive equality.

    \textit{Symmetry.}  We must prove that if $a_1b_2 = b_1a_2$, then $b_1a_2 =
    a_1b_2$.  This is true by the symmetry of equality.

    \textit{Transitivity.}  We must prove that if $a_1b_2 = b_1a_2$ and
    $b_1c_2 = c_1b_2$, then $a_1c_2 = c_1a_2$.
    \begin{align*}
        b_1a_2c_2 &= b_1c_2a_2 \\
        a_1b_2c_2 &= c_1b_2a_2 \\
        a_1c_2 &= c_1a_2,
    \end{align*}
    where the cancelling is valid because $b_2 \neq 0$ by definition.
\end{proof}

\begin{definition}
    Define the type $\Frac(\U)$ to be the type $(\U \times \U^*)/\sim$.
\end{definition}

We will use the notation $\frac{a}{b}$ to refer to $[(a, b)]$.  Once division is
defined we will see that this doesn't conflict with the usual fraction notation.

\begin{definition}
    Define the inclusion $\iota_\U : \U \to \frac(\U)$ that takes an $x : \U$
    and bring it to $\frac{x}{1}$.
\end{definition}

\begin{instance}
    $\iota_\U$ is injective.
\end{instance}
\begin{proof}
    If $\iota_\U(a) = \iota_\U(b)$, this means that $a1 = b1$, meaning that $a =
    b$.
\end{proof}

\begin{instance}
    $\Frac(\U)$ is not trivial.
\end{instance}
\begin{proof}
    Because $0 \neq 1$ in $\U$, by $\iota_\U$ being injective we have
    $\iota_\U(0) \neq \iota_\U(1)$.
\end{proof}

\section{Addition}

\begin{definition}
    Define an operation $\oplus : \U \times \U^* \to \U \times \U^* \to \U
    \times \U^*$ given by
    \[
        (a_1, a_2) \oplus (b_1, b_2) = (a_1b_2 + b_1a_2, a_2b_2).
    \]
    $a_2b_2$ is nonzero by Theorem \ref{mult_nz}.
\end{definition}

\begin{lemma}
    The operation $\oplus$ is well-defined under the equivalence relation
    $\sim$.
\end{lemma}
\begin{proof}
    We must prove that for all $a$, $b$, $c$, and $d$, if $a \sim b$ and $c \sim
    d$, we have $a \oplus c \sim b \oplus d$.  Thus, we have
    \[
        a_1b_2 = b_1a_2
    \]
    and
    \[
        c_1d_2 = d_1c_2
    \]
    and must prove that
    \[
        (a_1c_2 + c_1a_2)b_2d_2 = (b_1d_2 + d_1b_2)a_2c_2.
    \]
    Multiplying the first equation by $c_2d_2$ we get
    \[
        a_1c_2b_2d_2 = b_1d_2a_2c_2,
    \]
    and multiplying the second equation by $a_2b_2$ we get
    \[
        c_1a_2b_2d_2 = d_1b_2a_2c_2.
    \]
    Adding these two equations gives us
    \begin{align*}
        a_1c_2b_2d_2 + c_1a_2b_2d_2 &= b_1d_2a_2c_2 + d_1b_2a_2c_2 \\
        (a_1c_2 + c_1a_2)b_2d_2 &= (b_1d_2 + d_1b_2)a_2c_2
    \end{align*}
    as required.
\end{proof}

\begin{instance}
    Define addition in $\Frac(\U)$ as the binary operation given by Theorem
    \ref{binary_op_ex} and the previous lemma.
\end{instance}

\begin{instance}
    Addition in $\Frac(\U)$ is commutative.
\end{instance}
\begin{proof}
    \[
        a + b
        = \frac{a_1}{a_2} + \frac{b_1}{b_2}
        = \frac{a_1b_2 + b_1a_2}{a_2b_2}
        = \frac{b_1a_2 + a_1b_2}{b_2a_2}
        = \frac{b_1}{b_2} + \frac{a_1}{a_2}
        = b + a.
    \]
\end{proof}

\begin{instance}
    Addition in $\Frac(\U)$ is associative.
\end{instance}
\begin{proof}
    \begin{align*}
        a + (b + c)
        &= \frac{a_1}{a_2} + \left( \frac{b_1}{b_2} + \frac{c_1}{c_2} \right) \\
        &= \frac{a_1}{a_2} + \frac{b_1c_2 + c_1b_2}{b_2c_2} \\
        &= \frac{a_1(b_2c_2) + (b_1c_2 + c_1b_2)a_2}{a_2b_2c_2} \\
        &= \frac{a_1b_2c_2 + a_2b_1c_2 + a_2b_2c_1}{a_2b_2c_2} \\
        &= \frac{(a_1b_2 + b_1a_2)c_2 + c_1(a_2b_2)}{a_2b_2c_2} \\
        &= \frac{a_1b_2 + b_1a_2}{a_2b_2} + \frac{c_1}{c_2} \\
        &= \left( \frac{a_1}{a_2} + \frac{b_1}{b_2} \right) \frac{c_1}{c_2} \\
        &= (a + b) + c.
    \end{align*}
\end{proof}

\begin{instance}
    Define zero in $\Frac(\U)$ as $\iota_\U(0)$.
\end{instance}

\begin{instance}
    Zero is an additive identity in $\Frac(\U)$.
\end{instance}
\begin{proof}
    \[
        0 + a =
        \frac{0}{1} + \frac{a_1}{a_2} =
        \frac{0a_2 + a_11}{1a_2} =
        \frac{a_1}{a_2} =
        = a.
    \]
\end{proof}

\begin{definition}
    Define an operation $\ominus : \U \times \U^* \to \U \times \U^*$ given by
    \[
        \ominus (a_1, a_2) = (-a_1, a_2).
    \]
\end{definition}

\begin{lemma}
    The operation $\ominus$ is well-defined.
\end{lemma}
\begin{proof}
    We must prove that $a_1b_2 = b_1a_2$ implies $-a_1b_2 = -b_1a_2$, which can
    be done just by finding the negative of both sides.
\end{proof}

\begin{instance}
    Define additive inverses in $\Frac(\U)$ as the operation given by Theorem
    \ref{unary_op_ex} and the previous lemma.
\end{instance}

\begin{instance}
    Negation is a left inverse in $\Frac(\U)$.
\end{instance}
\begin{proof}
    For all $a$,
    \[
        a - a =
        \frac{a_1}{a_2} + \frac{-a_1}{a_2} =
        \frac{a_1a_2 - a_1a_2}{a_2a_2} =
        \frac{0}{a_2a_2} =
        \frac{0}{1} =
        0.
    \]
\end{proof}

\begin{instance}
    $\iota_\U$ is additive.
\end{instance}
\begin{proof}
    \[
        \iota_\U(a + b) =
        \frac{a + b}{1} =
        \frac{a1 + b1}{(1)(1)} =
        \frac{a}{1} + \frac{b}{1} =
        \iota_\U(a) + \iota_\U(b).
    \]
\end{proof}

\section{Multiplication}

\begin{definition}
    Define an operation $\otimes : \U \times \U^* \to \U \times \U^* \to \U
    \times \U^*$ given by
    \[
        (a_1, a_2) \otimes (b_1, b_2) = (a_1b_1, a_2b_2).
    \]
    $a_2b_2$ is nonzero by Theorem \ref{mult_nz}.
\end{definition}

\begin{lemma}
    The operation $\otimes$ is well-defined under the equivalence relation
    $\sim$.
\end{lemma}
\begin{proof}
    We must prove that for all $a$, $b$, $c$, and $d$, if $a \sim b$ and $c \sim
    d$, we have $a \otimes c \sim b \otimes d$.  Thus, we have
    \[
        a_1b_2 = b_1a_2
    \]
    and
    \[
        c_1d_2 = d_1c_2
    \]
    and must prove that
    \[
        a_1c_1b_2d_2 = b_1d_1a_2c_2.
    \]
    This follows directly by multiplying the previous two equations.
\end{proof}

\begin{instance}
    Define multiplication in $\Frac(\U)$ as the binary operation given by
    Theorem \ref{binary_op_ex} and the previous lemma.
\end{instance}

\begin{instance}
    Multiplication in $\Frac(\U)$ is commutative.
\end{instance}
\begin{proof}
    \[
        ab
        = \frac{a_1}{a_2} \, \frac{b_1}{b_2}
        = \frac{a_1b_1}{a_2b_2}
        = \frac{b_1a_1}{b_2a_2}
        = \frac{b_1}{b_2} \, \frac{a_1}{a_2}
        = ba.
    \]
\end{proof}

\begin{instance}
    Multiplication in $\Frac(\U)$ is associative.
\end{instance}
\begin{proof}
    \[
        a(bc)
        = \frac{a_1}{a_2} \left( \frac{b_1}{b_2} \, \frac{c_1}{c_2} \right)
        = \frac{a_1}{a_2} \, \frac{b_1c_1}{b_2c_2}
        = \frac{a_1b_1c_1}{a_2b_2c_2}
        = \frac{a_1b_1}{a_2b_2} \, \frac{c_1}{c_2}
        = \left( \frac{a_1}{a_2} \, \frac{b_1}{b_2} \right) \frac{c_1}{c_2}
        = (ab)c.
    \]
\end{proof}

\begin{instance}
    Multiplication in $\Frac(\U)$ distributes over addition.
\end{instance}
\begin{proof}
    \begin{align*}
        a(b + c)
        &= \frac{a_1}{a_2} \left( \frac{b_1}{b_2} + \frac{c_1}{c_2} \right) \\
        &= \frac{a_1}{a_2} \, \frac{b_1c_2 + c_1b_2}{b_2c_2} \\
        &= \frac{a_1(b_1c_2 + c_1b_2)}{a_2b_2c_2} \\
        &= \frac{a_1b_1c_2 + a_1c_1b_2}{a_2b_2c_2} \\
        &= \frac{a_2(a_1b_1c_2 + a_1c_1b_2)}{a_2(a_2b_2c_2)} \\
        &= \frac{a_1b_1a_2c_2 + a_1c_1a_2b_2}{a_2b_2a_2c_2} \\
        &= \frac{a_1b_1}{a_2b_2} + \frac{a_1c_1}{a_2c_2} \\
        &= \frac{a_1}{a_2} \, \frac{b_1}{b_2}
            + \frac{a_1}{a_2} \, \frac{c_1}{c_2} \\
        &= ab + ac
    \end{align*}
\end{proof}

\begin{instance}
    Define one in $\Frac(\U)$ as $\iota_\U(1)$.
\end{instance}

\begin{instance}
    One is a multiplicative identity in $\Frac(\U)$.
\end{instance}
\begin{proof}
    \[
        1a
        = \frac{1}{1} \, \frac{a_1}{a_2}
        = \frac{1a_1}{1a_2}
        = \frac{a_1}{a_2}
        = a.
    \]
\end{proof}

\begin{definition}
    Define an operation $\oslash : \U \times \U^* \to \U \times \U^*$ given by
    \[
        \oslash(a_1, a_2) = \begin{cases}
            (a_1, a_2) \text{ if $a_1 = 0$} \\
            (a_2, a_1) \text{ if $a_1 \neq 0$}.
        \end{cases}
    \]
\end{definition}

\begin{lemma}
    The operation $\oslash$ is well-defined.
\end{lemma}
\begin{proof}
    We must prove that if $a \sim b$, then $\oslash a \sim \oslash b$.  There
    will be four cases, depending on if $a_1 = 0$ and $b_1 = 0$.  By symmetry
    the cases $a_1 = 0$, $b_1 \neq 0$ and $a_1 \neq 0$, $b_1 = 0$ are the same,
    so there are three cases.  In each case we have $a_1b_2 = b_1a_2$.
    \begin{case} $a_1 = 0$, $b_1 = 0$.
        In this case we just need to prove that $a \sim b$, which is what we
        started with.
    \end{case}
    \begin{case} $a_1 = 0$, $b_1 \neq 0$.
        From $a_1 = 0$ and $a_1b_2 = b_1a_2$, we see that $0 = b_1a_2$.
        However, this case has $b_1 \neq 0$, and $a_2 \neq 0$ by definition, so
        this is a contradiction.  Thus, this case is impossible.
    \end{case}
    \begin{case} $a_1 \neq 0$, $b_1 \neq 0$.
        We must prove that $a_2b_1 = b_2a_1$.  This is essentially the same as
        what we started with, $a_1b_2 = b_1a_2$.
    \end{case}
\end{proof}

\begin{definition}
    Define multiplicative inverses as the operation produced by Theorem
    \ref{unary_op_ex} and the previous lemma.
\end{definition}

\begin{instance}
    The reciprocal in $\Frac(\U)$ is a multiplicative inverse.
\end{instance}
\begin{proof}
    Let $a \neq 0$.  This means that $a_1 \neq 0$.  Then
    \[
        a a^{-1} = \frac{a_1}{a_2} \, \frac{a_2}{a_1}
        = \frac{a_1a_2}{a_2a_1}
        = \frac{1}{1}
        = 1.
    \]
\end{proof}

\begin{instance}
    $\iota_\U$ is multiplicative.
\end{instance}
\begin{proof}
    \[
        \iota_\U(ab)
        = \frac{ab}{1}
        = \frac{ab}{(1)(1)}
        = \frac{a}{1} \, \frac{b}{1}
        = \iota_\U(a) \iota_\U(b).
    \]
\end{proof}

\begin{instance}
    $\iota_\U$ preserves the multiplicative identity.
\end{instance}
\begin{proof}
    This was simply the definition of $1$ in $\Frac(\U)$.
\end{proof}

We can now show that the notation $\frac{a}{b}$ is consistent with our usual use
of division:

\begin{theorem}
    For all $a$ and $b$, $[(a, b)] = \iota_\U(a) \iota_\U(b)^{-1}$
\end{theorem}
\begin{proof}
    By assumption we have $b \neq 0$.  Thus,
    \[
        \iota_\U(a) \iota_\U(b)^{-1}
        = [(a, 1)] [(b, 1)]^{-1}
        = [(a, 1)] [(1, b)]
        = [(a, b)].
    \]
\end{proof}

Note that this theorem also implies that for all $x : \Frac(\U)$, there exist
values $a$ and $b$ in $\U$ such that $x = \frac{a}{b}$.

\section{Order}

\section{The Frac functor}

\section{The Rationals}

\end{document}
